\subsection{Question 6} 
To verify that this constitutes a Lie algebra, since our operation $ * $ is associative, we need to verify that the Lie bracket is antisymmetric, linear and obeys the Jacobi identity. Antisymmetry is simple
\[ 
 	[ Y , X ] = Y * X - X * Y  =  - ( X* Y - Y *X )  = - [ X, Y ] \] Now, to show linearity, it's a matter of just expanding out the algebra. 
\begin{align*} 
	[ X, \al Y + \be Z ] & = X * ( \al Y + \be Z )  - ( \al Y + \be Z ) * X \\
				& = \alpha ( X * Y ) + \be X * Z - \al Y * X  - \be Z * X \\
				&= \al [ X, Y ] + \be [X, Z ] 
\end{align*} Thus, we have linearity in the second argument. The final this to do is to prove the Jacobi identity.
\begin{align*} 
	 [ X , [ Y , Z] ] & + [ Y , [ Z, X ]] + [ Z, [ X, Y ]] \\
	  & = X * [ Y , Z ]  - [ Y , Z ] *Z + Y * [ Z, X ] - [ Z, X] * Y + Z * [ X, Y ]  - [ X, Y ] * Z \\
	& = X * ( Y * Z - Z * Y )  - ( Y * Z - Z * Y ) * X + Y * ( Z * X - X * Z )   - ( Z  * X - X * Z ) * Y \\
	& +  Z* ( X * Y - Y * Z ) - ( X * Y - Y * X ) * Z \\
	 &  = X * ( Y * Z ) - X * ( Z * Y ) - ( Y * Z ) * Z + ( Z * Y ) * X + Y * ( Z * X ) - Y * ( X * Z ) \\
	 & - ( Z* X ) * Y + ( X* Y ) * Z + Z * ( X * Y  )  - Z * ( Y * X ) - ( X * Y ) * Z + ( Y * X ) * Z \\
	 & = 0 
\end{align*}
Our terms cancel in the last term since associativity allows us to move around the respective brackets. 

\pagebreak 
